moving steps to their resp. files

pulse/src/ocaml/plugin/generated/Pulse_Prover_IntroExists.ml
@@ -1,1 +1,497 @@
 open Prims
+let (k_intro_exists :
+  Pulse_Typing_Env.env ->
+    Pulse_Syntax_Base.universe ->
+      Pulse_Syntax_Base.binder ->
+        Pulse_Syntax_Base.vprop ->
+          Pulse_Syntax_Base.term ->
+            Pulse_Syntax_Base.vprop ->
+              ((unit, unit, unit, unit)
+                 Pulse_Prover_Common.continuation_elaborator,
+                unit) FStar_Tactics_Effect.tac_repr)
+  =
+  fun uu___5 ->
+    fun uu___4 ->
+      fun uu___3 ->
+        fun uu___2 ->
+          fun uu___1 ->
+            fun uu___ ->
+              (fun g ->
+                 fun u ->
+                   fun b ->
+                     fun p ->
+                       fun e ->
+                         fun frame ->
+                           Obj.magic
+                             (FStar_Tactics_Effect.lift_div_tac
+                                (fun uu___ -> Prims.magic ()))) uu___5 uu___4
+                uu___3 uu___2 uu___1 uu___
+let (intro_exists :
+  Pulse_Prover_Common.preamble ->
+    unit Pulse_Prover_Common.prover_state ->
+      Pulse_Syntax_Base.universe ->
+        Pulse_Syntax_Base.binder ->
+          Pulse_Syntax_Base.vprop ->
+            Pulse_Syntax_Base.vprop Prims.list ->
+              unit ->
+                Pulse_Prover_Common.prover_t ->
+                  (unit Pulse_Prover_Common.prover_state, unit)
+                    FStar_Tactics_Effect.tac_repr)
+  =
+  fun preamble ->
+    fun pst ->
+      fun u ->
+        fun b ->
+          fun body ->
+            fun unsolved' ->
+              fun uu___ ->
+                fun prover ->
+                  FStar_Tactics_Effect.tac_bind
+                    (FStar_Sealed.seal
+                       (Obj.magic
+                          (FStar_Range.mk_range
+                             "Pulse.Prover.IntroExists.fst"
+                             (Prims.of_int (26)) (Prims.of_int (10))
+                             (Prims.of_int (26)) (Prims.of_int (22)))))
+                    (FStar_Sealed.seal
+                       (Obj.magic
+                          (FStar_Range.mk_range
+                             "Pulse.Prover.IntroExists.fst"
+                             (Prims.of_int (26)) (Prims.of_int (25))
+                             (Prims.of_int (195)) (Prims.of_int (6)))))
+                    (FStar_Tactics_Effect.lift_div_tac
+                       (fun uu___1 ->
+                          Pulse_Typing_Env.fresh pst.Pulse_Prover_Common.pg))
+                    (fun uu___1 ->
+                       (fun x ->
+                          Obj.magic
+                            (FStar_Tactics_Effect.tac_bind
+                               (FStar_Sealed.seal
+                                  (Obj.magic
+                                     (FStar_Range.mk_range
+                                        "Pulse.Prover.IntroExists.fst"
+                                        (Prims.of_int (27))
+                                        (Prims.of_int (11))
+                                        (Prims.of_int (27))
+                                        (Prims.of_int (29)))))
+                               (FStar_Sealed.seal
+                                  (Obj.magic
+                                     (FStar_Range.mk_range
+                                        "Pulse.Prover.IntroExists.fst"
+                                        (Prims.of_int (27))
+                                        (Prims.of_int (32))
+                                        (Prims.of_int (195))
+                                        (Prims.of_int (6)))))
+                               (FStar_Tactics_Effect.lift_div_tac
+                                  (fun uu___1 ->
+                                     ((b.Pulse_Syntax_Base.binder_ppname), x)))
+                               (fun uu___1 ->
+                                  (fun px ->
+                                     Obj.magic
+                                       (FStar_Tactics_Effect.tac_bind
+                                          (FStar_Sealed.seal
+                                             (Obj.magic
+                                                (FStar_Range.mk_range
+                                                   "Pulse.Prover.IntroExists.fst"
+                                                   (Prims.of_int (29))
+                                                   (Prims.of_int (4))
+                                                   (Prims.of_int (32))
+                                                   (Prims.of_int (74)))))
+                                          (FStar_Sealed.seal
+                                             (Obj.magic
+                                                (FStar_Range.mk_range
+                                                   "Pulse.Prover.IntroExists.fst"
+                                                   (Prims.of_int (34))
+                                                   (Prims.of_int (37))
+                                                   (Prims.of_int (195))
+                                                   (Prims.of_int (6)))))
+                                          (FStar_Tactics_Effect.lift_div_tac
+                                             (fun uu___1 ->
+                                                {
+                                                  Pulse_Prover_Common.g0 =
+                                                    (pst.Pulse_Prover_Common.pg);
+                                                  Pulse_Prover_Common.ctxt =
+                                                    (Pulse_Prover_Common.op_Star
+                                                       (Pulse_Checker_VPropEquiv.list_as_vprop
+                                                          pst.Pulse_Prover_Common.remaining_ctxt)
+                                                       (Pulse_Prover_Common.op_Array_Access
+                                                          pst.Pulse_Prover_Common.ss
+                                                          pst.Pulse_Prover_Common.solved));
+                                                  Pulse_Prover_Common.ctxt_typing
+                                                    = ();
+                                                  Pulse_Prover_Common.goals =
+                                                    (Pulse_Prover_Common.op_Star
+                                                       (Pulse_Prover_Common.op_Star
+                                                          pst.Pulse_Prover_Common.solved
+                                                          (Pulse_Syntax_Naming.open_term_nv
+                                                             body px))
+                                                       (Pulse_Checker_VPropEquiv.list_as_vprop
+                                                          unsolved'))
+                                                }))
+                                          (fun uu___1 ->
+                                             (fun preamble_sub ->
+                                                Obj.magic
+                                                  (FStar_Tactics_Effect.tac_bind
+                                                     (FStar_Sealed.seal
+                                                        (Obj.magic
+                                                           (FStar_Range.mk_range
+                                                              "Pulse.Prover.IntroExists.fst"
+                                                              (Prims.of_int (36))
+                                                              (Prims.of_int (4))
+                                                              (Prims.of_int (44))
+                                                              (Prims.of_int (20)))))
+                                                     (FStar_Sealed.seal
+                                                        (Obj.magic
+                                                           (FStar_Range.mk_range
+                                                              "Pulse.Prover.IntroExists.fst"
+                                                              (Prims.of_int (45))
+                                                              (Prims.of_int (6))
+                                                              (Prims.of_int (195))
+                                                              (Prims.of_int (6)))))
+                                                     (FStar_Tactics_Effect.lift_div_tac
+                                                        (fun uu___1 ->
+                                                           {
+                                                             Pulse_Prover_Common.pg
+                                                               =
+                                                               (pst.Pulse_Prover_Common.pg);
+                                                             Pulse_Prover_Common.remaining_ctxt
+                                                               =
+                                                               (Pulse_Checker_VPropEquiv.vprop_as_list
+                                                                  preamble_sub.Pulse_Prover_Common.ctxt);
+                                                             Pulse_Prover_Common.uvs
+                                                               =
+                                                               (pst.Pulse_Prover_Common.uvs);
+                                                             Pulse_Prover_Common.ss
+                                                               =
+                                                               (pst.Pulse_Prover_Common.ss);
+                                                             Pulse_Prover_Common.solved
+                                                               =
+                                                               Pulse_Syntax_Base.tm_emp;
+                                                             Pulse_Prover_Common.unsolved
+                                                               =
+                                                               (FStar_List_Tot_Base.append
+                                                                  (Pulse_Checker_VPropEquiv.vprop_as_list
+                                                                    (Pulse_Prover_Common.op_Array_Access
+                                                                    pst.Pulse_Prover_Common.ss
+                                                                    pst.Pulse_Prover_Common.solved))
+                                                                  (FStar_List_Tot_Base.append
+                                                                    [
+                                                                    Pulse_Syntax_Naming.open_term_nv
+                                                                    body px]
+                                                                    unsolved'));
+                                                             Pulse_Prover_Common.k
+                                                               =
+                                                               (Prims.magic
+                                                                  ());
+                                                             Pulse_Prover_Common.goals_inv
+                                                               = ();
+                                                             Pulse_Prover_Common.solved_inv
+                                                               = ()
+                                                           }))
+                                                     (fun uu___1 ->
+                                                        (fun pst_sub ->
+                                                           Obj.magic
+                                                             (FStar_Tactics_Effect.tac_bind
+                                                                (FStar_Sealed.seal
+                                                                   (Obj.magic
+                                                                    (FStar_Range.mk_range
+                                                                    "Pulse.Prover.IntroExists.fst"
+                                                                    (Prims.of_int (47))
+                                                                    (Prims.of_int (25))
+                                                                    (Prims.of_int (47))
+                                                                    (Prims.of_int (39)))))
+                                                                (FStar_Sealed.seal
+                                                                   (Obj.magic
+                                                                    (FStar_Range.mk_range
+                                                                    "Pulse.Prover.IntroExists.fst"
+                                                                    (Prims.of_int (47))
+                                                                    (Prims.of_int (42))
+                                                                    (Prims.of_int (195))
+                                                                    (Prims.of_int (6)))))
+                                                                (Obj.magic
+                                                                   (prover
+                                                                    preamble_sub
+                                                                    pst_sub))
+                                                                (fun uu___1
+                                                                   ->
+                                                                   (fun
+                                                                    pst_sub_terminal
+                                                                    ->
+                                                                    Obj.magic
+                                                                    (FStar_Tactics_Effect.tac_bind
+                                                                    (FStar_Sealed.seal
+                                                                    (Obj.magic
+                                                                    (FStar_Range.mk_range
+                                                                    "Pulse.Prover.IntroExists.fst"
+                                                                    (Prims.of_int (51))
+                                                                    (Prims.of_int (65))
+                                                                    (Prims.of_int (51))
+                                                                    (Prims.of_int (91)))))
+                                                                    (FStar_Sealed.seal
+                                                                    (Obj.magic
+                                                                    (FStar_Range.mk_range
+                                                                    "Pulse.Prover.IntroExists.fst"
+                                                                    (Prims.of_int (52))
+                                                                    (Prims.of_int (86))
+                                                                    (Prims.of_int (195))
+                                                                    (Prims.of_int (6)))))
+                                                                    (FStar_Tactics_Effect.lift_div_tac
+                                                                    (fun
+                                                                    uu___1 ->
+                                                                    ()))
+                                                                    (fun
+                                                                    uu___1 ->
+                                                                    (fun
+                                                                    pst_sub_terminal_goals_inv
+                                                                    ->
+                                                                    Obj.magic
+                                                                    (FStar_Tactics_Effect.tac_bind
+                                                                    (FStar_Sealed.seal
+                                                                    (Obj.magic
+                                                                    (FStar_Range.mk_range
+                                                                    "Pulse.Prover.IntroExists.fst"
+                                                                    (Prims.of_int (57))
+                                                                    (Prims.of_int (66))
+                                                                    (Prims.of_int (57))
+                                                                    (Prims.of_int (74)))))
+                                                                    (FStar_Sealed.seal
+                                                                    (Obj.magic
+                                                                    (FStar_Range.mk_range
+                                                                    "Pulse.Prover.IntroExists.fst"
+                                                                    (Prims.of_int (57))
+                                                                    (Prims.of_int (77))
+                                                                    (Prims.of_int (195))
+                                                                    (Prims.of_int (6)))))
+                                                                    (FStar_Tactics_Effect.lift_div_tac
+                                                                    (fun
+                                                                    uu___1 ->
+                                                                    ()))
+                                                                    (fun
+                                                                    uu___1 ->
+                                                                    (fun
+                                                                    pst_sub_terminal_goals_inv1
+                                                                    ->
+                                                                    Obj.magic
+                                                                    (FStar_Tactics_Effect.tac_bind
+                                                                    (FStar_Sealed.seal
+                                                                    (Obj.magic
+                                                                    (FStar_Range.mk_range
+                                                                    "Pulse.Prover.IntroExists.fst"
+                                                                    (Prims.of_int (61))
+                                                                    (Prims.of_int (4))
+                                                                    (Prims.of_int (61))
+                                                                    (Prims.of_int (22)))))
+                                                                    (FStar_Sealed.seal
+                                                                    (Obj.magic
+                                                                    (FStar_Range.mk_range
+                                                                    "Pulse.Prover.IntroExists.fst"
+                                                                    (Prims.of_int (61))
+                                                                    (Prims.of_int (25))
+                                                                    (Prims.of_int (195))
+                                                                    (Prims.of_int (6)))))
+                                                                    (FStar_Tactics_Effect.lift_div_tac
+                                                                    (fun
+                                                                    uu___1 ->
+                                                                    pst_sub_terminal.Pulse_Prover_Common.k))
+                                                                    (fun
+                                                                    uu___1 ->
+                                                                    (fun
+                                                                    k_sub_terminal
+                                                                    ->
+                                                                    Obj.magic
+                                                                    (FStar_Tactics_Effect.tac_bind
+                                                                    (FStar_Sealed.seal
+                                                                    (Obj.magic
+                                                                    (FStar_Range.mk_range
+                                                                    "Pulse.Prover.IntroExists.fst"
+                                                                    (Prims.of_int (67))
+                                                                    (Prims.of_int (4))
+                                                                    (Prims.of_int (67))
+                                                                    (Prims.of_int (12)))))
+                                                                    (FStar_Sealed.seal
+                                                                    (Obj.magic
+                                                                    (FStar_Range.mk_range
+                                                                    "Pulse.Prover.IntroExists.fst"
+                                                                    (Prims.of_int (67))
+                                                                    (Prims.of_int (15))
+                                                                    (Prims.of_int (195))
+                                                                    (Prims.of_int (6)))))
+                                                                    (FStar_Tactics_Effect.lift_div_tac
+                                                                    (fun
+                                                                    uu___1 ->
+                                                                    Prims.magic
+                                                                    ()))
+                                                                    (fun
+                                                                    uu___1 ->
+                                                                    (fun
+                                                                    k_sub_terminal1
+                                                                    ->
+                                                                    Obj.magic
+                                                                    (FStar_Tactics_Effect.tac_bind
+                                                                    (FStar_Sealed.seal
+                                                                    (Obj.magic
+                                                                    (FStar_Range.mk_range
+                                                                    "Pulse.Prover.IntroExists.fst"
+                                                                    (Prims.of_int (74))
+                                                                    (Prims.of_int (4))
+                                                                    (Prims.of_int (74))
+                                                                    (Prims.of_int (18)))))
+                                                                    (FStar_Sealed.seal
+                                                                    (Obj.magic
+                                                                    (FStar_Range.mk_range
+                                                                    "Pulse.Prover.IntroExists.fst"
+                                                                    (Prims.of_int (77))
+                                                                    (Prims.of_int (137))
+                                                                    (Prims.of_int (195))
+                                                                    (Prims.of_int (6)))))
+                                                                    (FStar_Tactics_Effect.lift_div_tac
+                                                                    (fun
+                                                                    uu___1 ->
+                                                                    k_sub_terminal1))
+                                                                    (fun
+                                                                    uu___1 ->
+                                                                    (fun
+                                                                    k_sub_terminal2
+                                                                    ->
+                                                                    Obj.magic
+                                                                    (FStar_Tactics_Effect.tac_bind
+                                                                    (FStar_Sealed.seal
+                                                                    (Obj.magic
+                                                                    (FStar_Range.mk_range
+                                                                    "Pulse.Prover.IntroExists.fst"
+                                                                    (Prims.of_int (78))
+                                                                    (Prims.of_int (16))
+                                                                    (Prims.of_int (78))
+                                                                    (Prims.of_int (48)))))
+                                                                    (FStar_Sealed.seal
+                                                                    (Obj.magic
+                                                                    (FStar_Range.mk_range
+                                                                    "Pulse.Prover.IntroExists.fst"
+                                                                    (Prims.of_int (78))
+                                                                    (Prims.of_int (51))
+                                                                    (Prims.of_int (195))
+                                                                    (Prims.of_int (6)))))
+                                                                    (FStar_Tactics_Effect.lift_div_tac
+                                                                    (fun
+                                                                    uu___1 ->
+                                                                    Pulse_Prover_Common.op_Array_Access
+                                                                    pst_sub_terminal.Pulse_Prover_Common.ss
+                                                                    (Pulse_Syntax_Pure.null_var
+                                                                    x)))
+                                                                    (fun
+                                                                    uu___1 ->
+                                                                    (fun
+                                                                    witness
+                                                                    ->
+                                                                    Obj.magic
+                                                                    (FStar_Tactics_Effect.tac_bind
+                                                                    (FStar_Sealed.seal
+                                                                    (Obj.magic
+                                                                    (FStar_Range.mk_range
+                                                                    "Pulse.Prover.IntroExists.fst"
+                                                                    (Prims.of_int (87))
+                                                                    (Prims.of_int (89))
+                                                                    (Prims.of_int (87))
+                                                                    (Prims.of_int (97)))))
+                                                                    (FStar_Sealed.seal
+                                                                    (Obj.magic
+                                                                    (FStar_Range.mk_range
+                                                                    "Pulse.Prover.IntroExists.fst"
+                                                                    (Prims.of_int (87))
+                                                                    (Prims.of_int (100))
+                                                                    (Prims.of_int (195))
+                                                                    (Prims.of_int (6)))))
+                                                                    (FStar_Tactics_Effect.lift_div_tac
+                                                                    (fun
+                                                                    uu___1 ->
+                                                                    Prims.magic
+                                                                    ()))
+                                                                    (fun
+                                                                    uu___1 ->
+                                                                    (fun
+                                                                    k_sub_terminal3
+                                                                    ->
+                                                                    Obj.magic
+                                                                    (FStar_Tactics_Effect.tac_bind
+                                                                    (FStar_Sealed.seal
+                                                                    (Obj.magic
+                                                                    (FStar_Range.mk_range
+                                                                    "Pulse.Prover.IntroExists.fst"
+                                                                    (Prims.of_int (98))
+                                                                    (Prims.of_int (4))
+                                                                    (Prims.of_int (101))
+                                                                    (Prims.of_int (53)))))
+                                                                    (FStar_Sealed.seal
+                                                                    (Obj.magic
+                                                                    (FStar_Range.mk_range
+                                                                    "Pulse.Prover.IntroExists.fst"
+                                                                    (Prims.of_int (184))
+                                                                    (Prims.of_int (4))
+                                                                    (Prims.of_int (192))
+                                                                    (Prims.of_int (26)))))
+                                                                    (Obj.magic
+                                                                    (k_intro_exists
+                                                                    pst_sub_terminal.Pulse_Prover_Common.pg
+                                                                    u
+                                                                    (Pulse_Prover_Substs.nt_subst_binder
+                                                                    b
+                                                                    (Pulse_Prover_Substs.as_nt_substs
+                                                                    pst_sub_terminal.Pulse_Prover_Common.ss))
+                                                                    (Pulse_Prover_Common.op_Array_Access
+                                                                    pst_sub_terminal.Pulse_Prover_Common.ss
+                                                                    body)
+                                                                    witness
+                                                                    (Pulse_Prover_Common.op_Star
+                                                                    (Pulse_Prover_Common.op_Star
+                                                                    (Pulse_Checker_VPropEquiv.list_as_vprop
+                                                                    pst_sub_terminal.Pulse_Prover_Common.remaining_ctxt)
+                                                                    (Pulse_Prover_Common.op_Array_Access
+                                                                    pst_sub_terminal.Pulse_Prover_Common.ss
+                                                                    pst.Pulse_Prover_Common.solved))
+                                                                    (Pulse_Prover_Common.op_Array_Access
+                                                                    pst_sub_terminal.Pulse_Prover_Common.ss
+                                                                    (Pulse_Checker_VPropEquiv.list_as_vprop
+                                                                    unsolved')))))
+                                                                    (fun
+                                                                    k_intro_exists1
+                                                                    ->
+                                                                    FStar_Tactics_Effect.lift_div_tac
+                                                                    (fun
+                                                                    uu___1 ->
+                                                                    {
+                                                                    Pulse_Prover_Common.pg
+                                                                    =
+                                                                    (pst_sub_terminal.Pulse_Prover_Common.pg);
+                                                                    Pulse_Prover_Common.remaining_ctxt
+                                                                    =
+                                                                    (pst_sub_terminal.Pulse_Prover_Common.remaining_ctxt);
+                                                                    Pulse_Prover_Common.uvs
+                                                                    =
+                                                                    (pst_sub_terminal.Pulse_Prover_Common.uvs);
+                                                                    Pulse_Prover_Common.ss
+                                                                    =
+                                                                    (pst_sub_terminal.Pulse_Prover_Common.ss);
+                                                                    Pulse_Prover_Common.solved
+                                                                    =
+                                                                    (preamble.Pulse_Prover_Common.goals);
+                                                                    Pulse_Prover_Common.unsolved
+                                                                    = [];
+                                                                    Pulse_Prover_Common.k
+                                                                    =
+                                                                    (Prims.magic
+                                                                    ());
+                                                                    Pulse_Prover_Common.goals_inv
+                                                                    = ();
+                                                                    Pulse_Prover_Common.solved_inv
+                                                                    = ()
+                                                                    }))))
+                                                                    uu___1)))
+                                                                    uu___1)))
+                                                                    uu___1)))
+                                                                    uu___1)))
+                                                                    uu___1)))
+                                                                    uu___1)))
+                                                                    uu___1)))
+                                                                    uu___1)))
+                                                          uu___1))) uu___1)))
+                                    uu___1))) uu___1)
