pulse/src/ocaml/plugin/generated/Pulse_Prover_Match.ml
@@ -1,0 +1,115 @@
+open Prims
+let (try_match_pq :
+  Pulse_Typing_Env.env ->
+    Pulse_Typing_Env.env ->
+      Pulse_Syntax_Base.vprop ->
+        unit ->
+          Pulse_Syntax_Base.vprop ->
+            unit ->
+              ((Pulse_Prover_Substs.t, unit) Prims.dtuple2
+                 FStar_Pervasives_Native.option,
+                unit) FStar_Tactics_Effect.tac_repr)
+  =
+  fun uu___5 ->
+    fun uu___4 ->
+      fun uu___3 ->
+        fun uu___2 ->
+          fun uu___1 ->
+            fun uu___ ->
+              (fun g ->
+                 fun uvs ->
+                   fun p ->
+                     fun p_typing ->
+                       fun q ->
+                         fun q_typing ->
+                           Obj.magic
+                             (FStar_Tactics_Effect.lift_div_tac
+                                (fun uu___ -> Prims.magic ()))) uu___5 uu___4
+                uu___3 uu___2 uu___1 uu___
+let (compose_ss :
+  Pulse_Prover_Substs.t -> Pulse_Prover_Substs.t -> Pulse_Prover_Substs.t) =
+  fun ss1 -> fun ss2 -> Prims.magic ()
+let (match_step :
+  Pulse_Prover_Common.preamble ->
+    unit Pulse_Prover_Common.prover_state ->
+      Pulse_Syntax_Base.vprop ->
+        Pulse_Syntax_Base.vprop Prims.list ->
+          Pulse_Syntax_Base.vprop ->
+            Pulse_Syntax_Base.vprop Prims.list ->
+              unit ->
+                (unit Pulse_Prover_Common.prover_state
+                   FStar_Pervasives_Native.option,
+                  unit) FStar_Tactics_Effect.tac_repr)
+  =
+  fun preamble ->
+    fun pst ->
+      fun p ->
+        fun remaining_ctxt' ->
+          fun q ->
+            fun unsolved' ->
+              fun uu___ ->
+                FStar_Tactics_Effect.tac_bind
+                  (FStar_Sealed.seal
+                     (Obj.magic
+                        (FStar_Range.mk_range "Pulse.Prover.Match.fst"
+                           (Prims.of_int (28)) (Prims.of_int (11))
+                           (Prims.of_int (28)) (Prims.of_int (21)))))
+                  (FStar_Sealed.seal
+                     (Obj.magic
+                        (FStar_Range.mk_range "Pulse.Prover.Match.fst"
+                           (Prims.of_int (29)) (Prims.of_int (52))
+                           (Prims.of_int (91)) (Prims.of_int (11)))))
+                  (FStar_Tactics_Effect.lift_div_tac
+                     (fun uu___1 ->
+                        Pulse_Prover_Common.op_Array_Access
+                          pst.Pulse_Prover_Common.ss q))
+                  (fun uu___1 ->
+                     (fun q_ss ->
+                        Obj.magic
+                          (FStar_Tactics_Effect.tac_bind
+                             (FStar_Sealed.seal
+                                (Obj.magic
+                                   (FStar_Range.mk_range
+                                      "Pulse.Prover.Match.fst"
+                                      (Prims.of_int (31)) (Prims.of_int (11))
+                                      (Prims.of_int (31)) (Prims.of_int (69)))))
+                             (FStar_Sealed.seal
+                                (Obj.magic
+                                   (FStar_Range.mk_range
+                                      "Pulse.Prover.Match.fst"
+                                      (Prims.of_int (32)) Prims.int_zero
+                                      (Prims.of_int (91)) (Prims.of_int (11)))))
+                             (Obj.magic
+                                (try_match_pq pst.Pulse_Prover_Common.pg
+                                   pst.Pulse_Prover_Common.uvs p () q_ss ()))
+                             (fun ropt ->
+                                FStar_Tactics_Effect.lift_div_tac
+                                  (fun uu___1 ->
+                                     match ropt with
+                                     | FStar_Pervasives_Native.None ->
+                                         FStar_Pervasives_Native.None
+                                     | FStar_Pervasives_Native.Some
+                                         (Prims.Mkdtuple2 (ss_q, veq)) ->
+                                         FStar_Pervasives_Native.Some
+                                           {
+                                             Pulse_Prover_Common.pg =
+                                               (pst.Pulse_Prover_Common.pg);
+                                             Pulse_Prover_Common.remaining_ctxt
+                                               = remaining_ctxt';
+                                             Pulse_Prover_Common.uvs =
+                                               (pst.Pulse_Prover_Common.uvs);
+                                             Pulse_Prover_Common.ss =
+                                               (compose_ss ss_q
+                                                  pst.Pulse_Prover_Common.ss);
+                                             Pulse_Prover_Common.solved =
+                                               (Pulse_Prover_Common.op_Star q
+                                                  pst.Pulse_Prover_Common.solved);
+                                             Pulse_Prover_Common.unsolved =
+                                               unsolved';
+                                             Pulse_Prover_Common.k =
+                                               (Prims.magic ());
+                                             Pulse_Prover_Common.goals_inv =
+                                               ();
+                                             Pulse_Prover_Common.solved_inv =
+                                               ()
+                                           })))) uu___1)
