pulse/lib/steel/pulse/Pulse.Prover.IntroExists.fsti
@@ -4,9 +4,12 @@ module T = FStar.Tactics
 
 open Pulse.Syntax
 open Pulse.Typing
-open Pulse.Checker.Common
-open Pulse.Typing.Metatheory
-open Pulse.Checker.VPropEquiv
 open Pulse.Prover.Common
 
-// val intro_exists_prover_step : prover_step_t
+val intro_exists (#preamble:_) (pst:prover_state preamble)
+  (u:universe) (b:binder) (body:vprop)
+  (unsolved':list vprop)
+  (_:squash (pst.unsolved == (tm_exists_sl u b body)::unsolved'))
+  (prover:prover_t)
+  : T.Tac (pst':prover_state preamble { pst' `pst_extends` pst /\
+                                        is_terminal pst' })
